backend/Asmgenproof0.v
@@ -789,6 +789,7 @@ Qed.
 
 Section STRAIGHTLINE.
 
+Variable pol: policy.
 Variable ge: genv.
 Variable cp: compartment.
 Variable fn: function.
@@ -862,15 +863,19 @@ Lemma exec_straight_steps_1:
   rs#PC = Vptr b ofs ->
   Genv.find_funct_ptr ge b = Some (Internal fn) ->
   code_tail (Ptrofs.unsigned ofs) (fn_code fn) c ->
-  plus step ge (State rs m) E0 (State rs' m').
+  plus (step pol) ge (State rs m) E0 (State rs' m').
 Proof.
   induction 1; intros.
   apply plus_one.
   econstructor; eauto.
   eapply find_instr_tail. eauto.
+  rewrite H0. rewrite H2. reflexivity.
+  left; auto.
   eapply plus_left'.
   econstructor; eauto.
   eapply find_instr_tail. eauto.
+  rewrite H0. rewrite H3. reflexivity.
+  left; auto.
   apply IHexec_straight with b (Ptrofs.add ofs Ptrofs.one).
   auto. rewrite H0. rewrite H3. reflexivity.
   auto.
